Print assumptions, use bi_scope, notation consistency, comments.

theories/BaseLogic.v
@@ -28,7 +28,7 @@
 
 From Coq Require Import Classes.Morphisms Classes.Morphisms_Prop
   Classes.RelationClasses Relations.Relation_Definitions Strings.String.
-From iris Require bi.derived_connectives bi.interface proofmode.tactics.
+From iris Require Export bi.derived_connectives bi.interface proofmode.tactics.
 From stdpp Require Import base.
 
 From Em Require Export Environment Open Instantiation Substitution Worlds.
@@ -41,27 +41,24 @@ Import world.notations.
 #[local] Arguments thick : simpl never.
 
 #[local] Notation "Q [ θ ]" := (fun _ θ' => Q _ (θ ⊙ θ'))
-  (at level 8, left associativity, format "Q [ θ ]") : box_scope.
-
-Declare Scope pred_scope.
-Delimit Scope pred_scope with P.
+  (at level 7, left associativity, format "Q [ θ ]") : box_scope.
 
 #[local] Notation "P [ θ ]" := (subst P θ)
-  (at level 8, left associativity, format "P [ θ ]") : pred_scope.
+  (at level 7, left associativity, format "P [ θ ]") : bi_scope.
 
 Module Pred.
 
   Definition Pred (w : World) : Type := Assignment w -> Prop.
-  Bind Scope pred_scope with Pred.
+  Bind Scope bi_scope with Pred.
 
   Section Definitions.
 
-    Definition eqₚ {T : OType} {A : Type} {instTA : Inst T A} : ⊧ T ⇢ T ⇢ Pred :=
+    Definition oeq {T : OType} {A : Type} {instTA : Inst T A} : ⊧ T ↠ T ↠ Pred :=
       fun w t1 t2 ι => inst t1 ι = inst t2 ι.
-    #[global] Arguments eqₚ {T A _} [w] _ _ _/.
-    Definition TPB : ⊧ OEnv ⇢ Const Exp ⇢ OTy ⇢ OExp ⇢ Pred :=
+    #[global] Arguments oeq {T A _} [w] _ _ _/.
+    Definition otyping_decl : ⊧ OEnv ↠ Const Exp ↠ OTy ↠ OExp ↠ Pred :=
       fun w G e t ee ι => inst G ι |-- e ∷ inst t ι ~> inst ee ι.
-    #[global] Arguments TPB [w] G e t ee ι/.
+    #[global] Arguments otyping_decl [w] G e t ee ι/.
 
     #[export] Instance subst_pred : Subst Pred :=
       fun Θ w1 P w2 θ ι2 => P (inst θ ι2).
@@ -102,8 +99,8 @@ Module Pred.
     Proof. firstorder. Qed.
 
   End RewriteRelations.
-  #[global] Arguments bientails {w} (_ _)%P.
-  #[global] Arguments entails {w} (_ _)%P.
+  #[global] Arguments bientails {w} (_ _)%I.
+  #[global] Arguments entails {w} (_ _)%I.
 
   Module Import proofmode.
 
@@ -162,54 +159,31 @@ Module Pred.
 
     Import iris.bi.interface iris.bi.derived_connectives.
 
-    Notation "P ⊣⊢ₚ Q" := (@equiv (bi_car (@bi_pred _)) (@pred_equiv _) P%P Q%P)
-      (at level 95).
-    Notation "(⊣⊢ₚ)" := (@equiv (bi_car (@bi_pred _)) (@pred_equiv _))
-      (only parsing).
-
-    Notation "P ⊢ₚ Q" := (@bi_entails (@bi_pred _) P%P Q%P) (at level 95).
-    Notation "(⊢ₚ)" := (@bi_entails (@bi_pred _)) (only parsing).
-
-    Notation "⊤ₚ" := (@bi_pure (@bi_pred _) True) : pred_scope.
-    Notation "⊥ₚ" := (@bi_pure (@bi_pred _) False) : pred_scope.
-    Notation "P <->ₚ Q" := (@bi_iff (@bi_pred _) P%P Q%P) (at level 94) : pred_scope.
-    Notation "P ->ₚ Q"  := (@bi_impl (@bi_pred _) P%P Q%P) (at level 94, right associativity) : pred_scope.
-    Notation "P /\ₚ Q"  := (@bi_and (@bi_pred _) P%P Q%P) (at level 80, right associativity) : pred_scope.
-    Notation "P \/ₚ Q"  := (@bi_or (@bi_pred _) P%P Q%P) (at level 85, right associativity) : pred_scope.
-
-    Infix "=ₚ" := eqₚ (at level 70, no associativity) : pred_scope.
-
-    Notation "∀ₚ x .. y , P" :=
-      (@bi_forall (@bi_pred _) _ (fun x => .. (@bi_forall (@bi_pred _) _ (fun y => P%P)) ..))
-      (at level 200, x binder, y binder, right associativity,
-        format "'[ ' '[ ' ∀ₚ  x .. y ']' ,  '/' P ']'") : pred_scope.
-    Notation "∃ₚ x .. y , P" :=
-      (@bi_exist (@bi_pred _) _ (fun x => .. (@bi_exist (@bi_pred _) _ (fun y => P%P)) ..))
-      (at level 200, x binder, y binder, right associativity,
-        format "'[ ' '[ ' ∃ₚ  x .. y ']' ,  '/' P ']'") : pred_scope.
-
+    Notation "⊤" := (@bi_pure (@bi_pred _) True) : bi_scope.
+    Notation "⊥" := (@bi_pure (@bi_pred _) False) : bi_scope.
+    Infix "≈" := oeq (at level 70, no associativity) : bi_scope.
     Notation "G |--ₚ E ; T ~> EE" :=
-      (TPB G E T EE) (at level 70, no associativity) : pred_scope.
+      (otyping_decl G E T EE) (at level 70, no associativity) : bi_scope.
 
   End notations.
 
   Lemma bientails_unfold [w] (P Q : Pred w) :
-    (P ⊣⊢ₚ Q) <-> forall ι, P ι <-> Q ι.
+    (P ⊣⊢ Q) <-> ∀ ι, P ι <-> Q ι.
   Proof. firstorder. Qed.
   Lemma entails_unfold [w] (P Q : Pred w) :
-    (P ⊢ₚ Q) <-> forall ι, P ι -> Q ι.
+    (P ⊢ Q) <-> ∀ ι, P ι -> Q ι.
   Proof. firstorder. Qed.
   Lemma sep_unfold w (P Q : Pred w) :
-    ∀ ι, interface.bi_sep P Q ι ↔ (P ι /\ Q ι).
+    ∀ ι, interface.bi_sep P Q ι ↔ (P ι ∧ Q ι).
   Proof. firstorder. Qed.
   Lemma wand_unfold w (P Q : Pred w) :
     ∀ ι, interface.bi_wand P Q ι ↔ (P ι → Q ι).
   Proof. firstorder. Qed.
   Lemma intuitionistically_unfold w (P : Pred w) :
-    ∀ ι, @derived_connectives.bi_intuitionistically _ P ι <-> P ι.
+    ∀ ι, @derived_connectives.bi_intuitionistically _ P ι ↔ P ι.
   Proof. firstorder. Qed.
 
-  Create HintDb punfold.
+  Create HintDb pred_unfold.
   #[export] Hint Rewrite bientails_unfold entails_unfold sep_unfold wand_unfold
     intuitionistically_unfold (@inst_subst OEnv Env _ _ _)
     (@inst_subst OExp Exp _ _ _) (@inst_subst OTy Ty _ _ _)
@@ -217,7 +191,7 @@ Module Pred.
     (@inst_lift OTy Ty _ _ _) (@inst_thin Par _ Par.lk_thin_par)
     @inst_refl @inst_trans @inst_insert @Open.inst_pure
     @oexp.inst_var @oexp.inst_true @oexp.inst_false @oexp.inst_ifte
-    @oexp.inst_absu @oexp.inst_abst @oexp.inst_app : punfold.
+    @oexp.inst_absu @oexp.inst_abst @oexp.inst_app : pred_unfold.
 
   Ltac punfold_connectives :=
     change (@interface.bi_and (@bi_pred _) ?P ?Q ?ι) with (P ι /\ Q ι) in *;
@@ -230,14 +204,13 @@ Module Pred.
     change (@subst Pred subst_pred _ _ ?P _ ?θ ?ι) with (P (inst θ ι)) in *;
     try progress (cbn beta).
 
+  (* A tactic that unfold all the predicates to expose the underlying
+      definitions. This is mainly used to finish proofs. *)
   Ltac pred_unfold :=
     repeat
       (punfold_connectives;
-       try rewrite_db punfold; auto 1 with typeclass_instances;
-       cbn [eqₚ TPB inst inst_ty inst_env] in *;
-       (* repeat rewrite ?inst_subst, ?inst_lift, ?inst_refl, ?inst_trans, *)
-       (*   ?inst_insert, ?oexp.inst_var, ?oexp.inst_true, ?oexp.inst_false, *)
-       (*   ?oexp.inst_absu, ?oexp.inst_abst, ?oexp.inst_app, ?oexp.inst_ifte in *; *)
+       try rewrite_db pred_unfold; auto 1 with typeclass_instances;
+       cbn [oeq otyping_decl inst inst_ty inst_env] in *;
        try
          match goal with
          | |- forall ι : Assignment _, _ =>
@@ -246,9 +219,6 @@ Module Pred.
              first [clear ι | revert ι]
          | |- @interface.bi_emp_valid (@bi_pred _) _ => constructor; intros ι _; cbn
          | |- @interface.bi_entails (@bi_pred _) _ _ => constructor; intros ι; cbn
-         (* | H: context[@inst ?AT ?A ?I ?w ?x ?ι] |- _ => *)
-         (*     is_var x; generalize (@inst AT A I w x ι); *)
-         (*     clear x; intro x; subst *)
          | |- context[@inst ?AT ?A ?I ?w ?x ?ι] =>
              is_var x; generalize (@inst AT A I w x ι);
              clear x; intro x; subst
@@ -265,16 +235,14 @@ Module Pred.
       repeat (autorewrite with obligation in *; cbn in *; intros; subst; pred_unfold);
       repeat
         (match goal with
-         | H: _ ⊢ₚ _ |- _ => destruct H as [H]
-         | H: _ ⊣⊢ₚ _ |- _ => destruct H as [H]
+         | H: _ ⊢ _ |- _ => destruct H as [H]
+         | H: _ ⊣⊢ _ |- _ => destruct H as [H]
          | H: forall (H : ?A), _, a : ?A |- _ =>
            specialize (H a); autorewrite with obligation in H; cbn in H
          | |- (forall _ : ?A, _) <-> (forall _ : ?A, _) =>
              apply all_iff_morphism; intro; autorewrite with obligation; cbn
          | |- (exists _ : ?A, _) <-> (exists _ : ?A, _) =>
              apply ex_iff_morphism; intro; autorewrite with obligation; cbn
-         (* | |- _ ⊣⊢ₚ _ => constructor; cbn; intros *)
-         (* | |- _ ⊢ₚ _ => constructor; cbn; intros *)
          end);
       try easy; try (intuition; fail); try (intuition congruence; fail).
     #[local] Obligation Tactic := obligation.
@@ -282,95 +250,94 @@ Module Pred.
     #[local] Hint Rewrite <- @tactics.forall_and_distr : obligation.
 
     #[export] Instance proper_subst_bientails {Θ w} :
-      Proper ((⊣⊢ₚ) ==> forall_relation (fun _ => eq ==> (⊣⊢ₚ)))
+      Proper ((⊣⊢) ==> forall_relation (fun _ => eq ==> (⊣⊢)))
       (@subst Pred Pred.subst_pred Θ w).
     Proof. obligation. Qed.
 
-    Lemma split_bientails {w} (P Q : Pred w) : (P ⊣⊢ₚ Q) <-> (P ⊢ₚ Q) /\ (Q ⊢ₚ P).
+    Lemma split_bientails {w} (P Q : Pred w) : (P ⊣⊢ Q) <-> (P ⊢ Q) ∧ (Q ⊢ P).
     Proof. obligation. Qed.
-    Lemma impl_and_adjoint {w} (P Q R : Pred w) : (P /\ₚ Q ⊢ₚ R) <-> (P ⊢ₚ Q ->ₚ R).
+    Lemma impl_and_adjoint {w} (P Q R : Pred w) : (P ∧ Q ⊢ R) <-> (P ⊢ Q → R).
     Proof. obligation. Qed.
-    Lemma and_true_l {w} (P : Pred w) : ⊤ₚ /\ₚ P ⊣⊢ₚ P.
+    Lemma and_true_l {w} (P : Pred w) : ⊤ ∧ P ⊣⊢ P.
     Proof. obligation. Qed.
-    Lemma and_true_r {w} (P : Pred w) : P /\ₚ ⊤ₚ ⊣⊢ₚ P.
+    Lemma and_true_r {w} (P : Pred w) : P ∧ ⊤ ⊣⊢ P.
     Proof. obligation. Qed.
-    Lemma and_false_l {w} (P : Pred w) : ⊥ₚ /\ₚ P ⊣⊢ₚ ⊥ₚ.
+    Lemma and_false_l {w} (P : Pred w) : ⊥ ∧ P ⊣⊢ ⊥.
     Proof. obligation. Qed.
-    Lemma and_false_r {w} (P : Pred w) : P /\ₚ ⊥ₚ ⊣⊢ₚ ⊥ₚ.
+    Lemma and_false_r {w} (P : Pred w) : P ∧ ⊥ ⊣⊢ ⊥.
     Proof. obligation. Qed.
-    Lemma impl_true_l {w} (P : Pred w) : ⊤ₚ ->ₚ P ⊣⊢ₚ P.
+    Lemma impl_true_l {w} (P : Pred w) : (⊤ → P) ⊣⊢ P.
     Proof. obligation. Qed.
-    Lemma impl_true_r {w} (P : Pred w) : P ->ₚ ⊤ₚ ⊣⊢ₚ ⊤ₚ.
+    Lemma impl_true_r {w} (P : Pred w) : (P → ⊤) ⊣⊢ ⊤.
     Proof. obligation. Qed.
-    Lemma impl_false_l {w} (P : Pred w) : ⊥ₚ ->ₚ P ⊣⊢ₚ ⊤ₚ.
+    Lemma impl_false_l {w} (P : Pred w) : (⊥ → P) ⊣⊢ ⊤.
     Proof. obligation. Qed.
-    (* Lemma false_l {w} (P : Pred w) : ⊥ₚ ⊢ₚ P. *)
+    (* Lemma false_l {w} (P : Pred w) : ⊥ ⊢ P. *)
     (* Proof. obligation. Qed. *)
-    (* Lemma true_r {w} (P : Pred w) : P ⊢ₚ ⊤ₚ. *)
+    (* Lemma true_r {w} (P : Pred w) : P ⊢ ⊤. *)
     (* Proof. obligation. Qed. *)
-    (* Lemma impl_forget {w} (P Q R : Pred w) : P ⊢ₚ R -> P ⊢ₚ (Q ->ₚ R). *)
+    (* Lemma impl_forget {w} (P Q R : Pred w) : (P ⊢ R) → (P ⊢ (Q → R)). *)
     (* Proof. obligation. Qed. *)
-    Lemma impl_and [w] (P Q R : Pred w) : ((P /\ₚ Q) ->ₚ R) ⊣⊢ₚ (P ->ₚ Q ->ₚ R).
+    Lemma impl_and [w] (P Q R : Pred w) : (P ∧ Q → R) ⊣⊢ (P → Q → R).
     Proof. obligation. Qed.
-
     (* Lemma forall_l {I : Type} {w} (P : I -> Pred w) Q : *)
-    (*   (exists x : I, P x ⊢ₚ Q) -> (∀ x : I, P x)%I ⊢ₚ Q. *)
+    (*   (∃ x : I, P x ⊢ Q) -> (∀ x : I, P x) ⊢ Q. *)
     (* Proof. obligation. firstorder. Qed. *)
     (* Lemma forall_r {I : Type} {w} P (Q : I -> Pred w) : *)
-    (*   (P ⊢ₚ (∀ₚ x : I, Q x)) <-> (forall x : I, P ⊢ₚ Q x). *)
+    (*   (P ⊢ (∀ x : I, Q x)) <-> (∀ x : I, (P ⊢ Q x)). *)
     (* Proof. obligation. firstorder. Qed. *)
 
     Lemma exists_l {I : Type} {w} (P : I -> Pred w) (Q : Pred w) :
-      (forall x : I, P x ⊢ₚ Q) -> (∃ₚ x : I, P x) ⊢ₚ Q.
+      (∀ x : I, P x ⊢ Q) -> (∃ x : I, P x) ⊢ Q.
     Proof. obligation; firstorder. Qed.
     Lemma exists_r {I : Type} {w} P (Q : I -> Pred w) :
-      (exists x : I, P ⊢ₚ Q x) -> P ⊢ₚ (∃ₚ x : I, Q x).
+      (∃ x : I, P ⊢ Q x) -> P ⊢ (∃ x : I, Q x).
     Proof. obligation; firstorder. Qed.
     #[global] Arguments exists_r {I w P Q} _.
 
-    Lemma wand_is_impl [w] (P Q : Pred w) : (P -∗ Q)%I ⊣⊢ₚ (P ->ₚ Q).
+    Lemma wand_is_impl [w] (P Q : Pred w) : (P -∗ Q) ⊣⊢ (P → Q).
     Proof. obligation. Qed.
 
-    Lemma pApply {w} {P Q R : Pred w} : P ⊢ₚ Q -> Q ⊢ₚ R -> P ⊢ₚ R.
+    Lemma pApply {w} {P Q R : Pred w} : (P ⊢ Q) -> (Q ⊢ R) -> (P ⊢ R).
     Proof. now transitivity Q. Qed.
 
-    Lemma pApply_r {w} {P Q R : Pred w} : Q ⊢ₚ R -> P ⊢ₚ Q -> P ⊢ₚ R.
+    Lemma pApply_r {w} {P Q R : Pred w} : (Q ⊢ R) → (P ⊢ Q) → (P ⊢ R).
     Proof. now transitivity Q. Qed.
 
     Section Eq.
 
       Context {T A} {instTA : Inst T A}.
 
-      Lemma eqₚ_intro {w} (t : T w) : ⊢ (t =ₚ t)%P.
+      Lemma oeq_intro {w} (t : T w) : ⊢ t ≈ t.
       Proof. obligation. Qed.
 
-      Lemma eqₚ_refl {w} (t : T w) : t =ₚ t ⊣⊢ₚ ⊤ₚ.
+      Lemma oeq_refl {w} (t : T w) : t ≈ t ⊣⊢ ⊤.
       Proof. obligation. Qed.
 
-      Lemma eqₚ_sym {w} (s t : T w) : s =ₚ t ⊣⊢ₚ t =ₚ s.
+      Lemma oeq_sym {w} (s t : T w) : s ≈ t ⊣⊢ t ≈ s.
       Proof. obligation. Qed.
 
-      Lemma eqₚ_trans {w} (s t u : T w) : s =ₚ t /\ₚ t =ₚ u ⊢ₚ s =ₚ u.
+      Lemma oeq_trans {w} (s t u : T w) : s ≈ t ∧ t ≈ u ⊢ s ≈ u.
       Proof. obligation. Qed.
 
     End Eq.
-    #[global] Arguments eqₚ_trans {T A _ w} s t u.
+    #[global] Arguments oeq_trans {T A _ w} s t u.
 
-    Lemma peq_ty_noconfusion {w} (t1 t2 : OTy w) :
-      t1 =ₚ t2 ⊣⊢ₚ
+    Lemma oeq_ty_noconfusion {w} (t1 t2 : OTy w) :
+      t1 ≈ t2 ⊣⊢
       match t1 , t2 with
-      | oty.evar  _      , _                => t1 =ₚ t2
-      | _                , oty.evar _       => t1 =ₚ t2
-      | oty.bool         , oty.bool         => ⊤ₚ
-      | oty.func t11 t12 , oty.func t21 t22 => t11 =ₚ t21 /\ₚ t12 =ₚ t22
-      | _                , _                => ⊥ₚ
+      | oty.evar  _      , _                => t1 ≈ t2
+      | _                , oty.evar _       => t1 ≈ t2
+      | oty.bool         , oty.bool         => True
+      | oty.func t11 t12 , oty.func t21 t22 => t11 ≈ t21 ∧ t12 ≈ t22
+      | _                , _                => False
       end.
     Proof. destruct t1, t2; obligation. Qed.
 
-    Lemma eq_pair
+    Lemma oeq_pair
       {AT BT : OType} {A B : Type} {instA : Inst AT A} {instB : Inst BT B}
       [w] (a1 a2 : AT w) (b1 b2 : BT w) :
-      (a1,b1) =ₚ (a2,b2) ⊣⊢ₚ ((a1 =ₚ a2) /\ₚ (b1 =ₚ b2)).
+      (a1,b1) ≈ (a2,b2) ⊣⊢ ((a1 ≈ a2) ∧ (b1 ≈ b2)).
     Proof.
       pred_unfold. intros ι; cbn. split.
       - now injection 1.
@@ -382,7 +349,7 @@ Module Pred.
       Lemma subst_eq {T : OType} {substT : Subst T}
         {A : Type} {instTA : Inst T A} {instSubstTA : InstSubst T A}
         {Θ : SUB} {w0 w1} (θ : Θ w0 w1) (t1 t2 : T w0) :
-        subst (t1 =ₚ t2) θ ⊣⊢ₚ subst t1 θ =ₚ subst t2 θ.
+        (t1 ≈ t2)[θ] ⊣⊢ t1[θ] ≈ t2[θ].
       Proof.
         pred_unfold. unfold subst, subst_pred. intros ι.
         now rewrite !inst_subst.
@@ -395,37 +362,36 @@ Module Pred.
          lemmas that use bientailment instead of Leibniz equality and thus
          avoid functional extensionality. *)
       Lemma subst_pred_refl `{lkReflΘ : LkRefl Θ} [w] (P : Pred w) :
-        subst P refl ⊣⊢ₚ P.
+        P[refl] ⊣⊢ P.
       Proof. obligation. Qed.
       Lemma subst_pred_trans `{lktransΘ : LkTrans Θ}
         {w0 w1 w2} (θ1 : Θ w0 w1) (θ2 : Θ w1 w2) (P : Pred w0) :
-        subst P (θ1 ⊙ θ2) ⊣⊢ₚ subst (subst P θ1) θ2.
+        P[θ1 ⊙ θ2] ⊣⊢ P[θ1][θ2].
       Proof. obligation. Qed.
       Lemma subst_and {w0 w1} (θ : Θ w0 w1) (P Q : Pred w0) :
-        subst (P /\ₚ Q) θ ⊣⊢ₚ subst P θ /\ₚ subst Q θ.
+        (P ∧ Q)[θ] ⊣⊢ P[θ] ∧ Q[θ].
       Proof. obligation. Qed.
       Lemma subst_impl {w0 w1} (θ : Θ w0 w1) (P Q : Pred w0) :
-        subst (P ->ₚ Q) θ ⊣⊢ₚ (subst P θ ->ₚ subst Q θ).
+        (P → Q)[θ] ⊣⊢ (P[θ] → Q[θ]).
       Proof. obligation. Qed.
       Lemma subst_wand {w0 w1} (θ : Θ w0 w1) (P Q : Pred w0) :
-        subst (interface.bi_wand P Q) θ ⊣⊢ₚ interface.bi_wand (subst P θ) (subst Q θ).
+        (P -∗ Q)[θ] ⊣⊢ (P[θ] -∗ Q[θ]).
       Proof. obligation. Qed.
       Lemma subst_false {w0 w1} (θ : Θ w0 w1) :
-        subst ⊥ₚ θ ⊣⊢ₚ ⊥ₚ.
+        ⊥[θ] ⊣⊢ ⊥.
       Proof. obligation. Qed.
       Lemma subst_true {w0 w1} (θ : Θ w0 w1) :
-        subst ⊤ₚ θ ⊣⊢ₚ ⊤ₚ.
+        ⊤[θ] ⊣⊢ ⊤.
       Proof. obligation. Qed.
       Lemma subst_forall [A] [w0 w1] (θ : Θ w0 w1) (Q : A -> Pred w0) :
-        subst (∀ₚ a : A, Q a) θ ⊣⊢ₚ (∀ₚ a : A, subst (Q a) θ).
+        (∀ a : A, Q a)[θ] ⊣⊢ (∀ a : A, (Q a)[θ]).
       Proof. obligation. Qed.
       Lemma subst_exists [A] [w0 w1] (θ : Θ w0 w1) (Q : A -> Pred w0) :
-        subst (∃ₚ a : A, Q a) θ ⊣⊢ₚ (∃ₚ a : A, subst (Q a) θ).
+        (∃ a : A, Q a)[θ] ⊣⊢ (∃ a : A, (Q a)[θ]).
       Proof. obligation. Qed.
 
-      Lemma subst_tpb {w0 w1} (θ : Θ w0 w1) G (e : Exp) (t : OTy w0) (ee : OExp w0) :
-        subst (G |--ₚ e; t ~> ee) θ ⊣⊢ₚ
-        subst G θ |--ₚ e; subst t θ ~> subst ee θ.
+      Lemma subst_typing {w0 w1} (θ : Θ w0 w1) G (e : Exp) (t : OTy w0) (ee : OExp w0) :
+        (G |--ₚ e; t ~> ee)[θ] ⊣⊢ G[θ] |--ₚ e; t[θ] ~> ee[θ].
       Proof. obligation. Qed.
 
     End Subst.
@@ -439,31 +405,31 @@ Module Pred.
       Context {Θ : SUB}.
 
       Definition wp {w0 w1} (θ : Θ w0 w1) (Q : Pred w1) : Pred w0 :=
-        fun ι0 => exists (ι1 : Assignment w1), inst θ ι1 = ι0 /\ Q ι1.
+        fun ι0 => exists (ι1 : Assignment w1), inst θ ι1 = ι0 ∧ Q ι1.
       Definition wlp {w0 w1} (θ : Θ w0 w1) (Q : Pred w1) : Pred w0 :=
-        fun ι0 => forall (ι1 : Assignment w1), inst θ ι1 = ι0 -> Q ι1.
+        fun ι0 => forall (ι1 : Assignment w1), inst θ ι1 = ι0 → Q ι1.
 
       #[global] Arguments wp {_ _} _ _ ι0/.
       #[global] Arguments wlp {_ _} _ _ ι0/.
 
       #[export] Instance proper_wp_bientails {w0 w1} (θ : Θ w0 w1) :
-        Proper ((⊣⊢ₚ) ==> (⊣⊢ₚ)) (wp θ).
+        Proper ((⊣⊢) ==> (⊣⊢)) (wp θ).
       Proof. firstorder. Qed.
 
       #[export] Instance proper_wp_entails {w0 w1} (θ : Θ w0 w1) :
-        Proper ((⊢ₚ) ==> (⊢ₚ)) (wp θ).
+        Proper ((⊢) ==> (⊢)) (wp θ).
       Proof. firstorder. Qed.
 
       #[export] Instance proper_wlp_bientails {w0 w1} (θ : Θ w0 w1) :
-        Proper ((⊣⊢ₚ) ==> (⊣⊢ₚ)) (wlp θ).
+        Proper ((⊣⊢) ==> (⊣⊢)) (wlp θ).
       Proof. firstorder. Qed.
 
       #[export] Instance proper_wlp_entails {w0 w1} (θ : Θ w0 w1) :
-        Proper ((⊢ₚ) ==> (⊢ₚ)) (wlp θ).
+        Proper ((⊢) ==> (⊢)) (wlp θ).
       Proof. firstorder. Qed.
 
       Lemma wp_refl {reflΘ : Refl Θ} {lkreflΘ : LkRefl Θ}
-        {w} (Q : Pred w) : wp refl Q ⊣⊢ₚ Q.
+        {w} (Q : Pred w) : wp refl Q ⊣⊢ Q.
       Proof.
         unfold wp; pred_unfold. intros ι; split.
         - intros (ι' & Heq & HQ). now subst.
@@ -472,7 +438,7 @@ Module Pred.
 
       Lemma wp_trans {transR : Trans Θ} {lktransΘ : LkTrans Θ}
         {w0 w1 w2} (θ1 : Θ w0 w1) (θ2 : Θ w1 w2) Q :
-        wp (θ1 ⊙ θ2) Q ⊣⊢ₚ wp θ1 (wp θ2 Q).
+        wp (θ1 ⊙ θ2) Q ⊣⊢ wp θ1 (wp θ2 Q).
       Proof.
         unfold wp; pred_unfold. intros ι; split.
         - intros (ι2 & Heq & HQ). eauto.
@@ -480,11 +446,11 @@ Module Pred.
       Qed.
 
       Lemma wp_false {w0 w1} (θ : Θ w0 w1) :
-        wp θ ⊥ₚ ⊣⊢ₚ ⊥ₚ.
+        wp θ ⊥ ⊣⊢ ⊥.
       Proof. firstorder. Qed.
 
       Lemma and_wp_l {w0 w1} (θ : Θ w0 w1) P Q :
-        wp θ P /\ₚ Q ⊣⊢ₚ wp θ (P /\ₚ subst Q θ).
+        wp θ P ∧ Q ⊣⊢ wp θ (P ∧ Q[θ]).
       Proof.
         unfold wp; pred_unfold. split.
         - intros [(ι1 & <- & HP) HQ]. eauto.
@@ -492,12 +458,12 @@ Module Pred.
       Qed.
 
       Lemma and_wp_r {w0 w1} (θ : Θ w0 w1) (P : Pred w0) (Q : Pred w1) :
-        P /\ₚ wp θ Q ⊣⊢ₚ wp θ (subst P θ /\ₚ Q).
+        P ∧ wp θ Q ⊣⊢ wp θ (P[θ] ∧ Q).
       Proof. now rewrite and_comm and_wp_l and_comm. Qed.
 
       Lemma wp_thick {thickΘ : Thick Θ} {lkThickΘ : LkThick Θ}
         {w α} (αIn : world.In α w) (t : OTy (w - α)) (Q : Pred (w - α)) :
-        wp (thick α t) Q ⊣⊢ₚ oty.evar αIn =ₚ subst t (thin (Θ := Par) α) /\ₚ subst Q (thin (Θ := Par) α).
+        wp (thick α t) Q ⊣⊢ oty.evar αIn ≈ t[thin (Θ := Par) α] ∧ Q[thin (Θ := Par) α].
       Proof.
         unfold wp; pred_unfold. intros ι. split.
         - intros (ι1 & Heq & HQ). subst.
@@ -507,7 +473,7 @@ Module Pred.
       Qed.
 
       Lemma wlp_refl {reflΘ : Refl Θ} {lkreflΘ : LkRefl Θ}
-        {w} (Q : Pred w) : wlp refl Q ⊣⊢ₚ Q.
+        {w} (Q : Pred w) : wlp refl Q ⊣⊢ Q.
       Proof.
         unfold wlp; pred_unfold. intros ι. split.
         - intros HQ. auto.
@@ -516,7 +482,7 @@ Module Pred.
 
       Lemma wlp_trans {transR : Trans Θ} {lktransΘ : LkTrans Θ}
         {w0 w1 w2} (θ1 : Θ w0 w1) (θ2 : Θ w1 w2) Q :
-        wlp (θ1 ⊙ θ2) Q ⊣⊢ₚ wlp θ1 (wlp θ2 Q).
+        wlp (θ1 ⊙ θ2) Q ⊣⊢ wlp θ1 (wlp θ2 Q).
       Proof.
         unfold wlp; pred_unfold. intros ι. split.
         - intros HQ ι1 Heq1 ι2 Heq2. subst; auto.
@@ -524,27 +490,27 @@ Module Pred.
       Qed.
 
       Lemma wlp_true {w0 w1} (θ : Θ w0 w1) :
-        wlp θ ⊤ₚ ⊣⊢ₚ ⊤ₚ.
+        wlp θ ⊤ ⊣⊢ ⊤.
       Proof. firstorder. Qed.
 
       (* Lemma wlp_and {w0 w1} (θ : Θ w0 w1) P Q : *)
-      (*   wlp θ P /\ₚ wlp θ Q ⊣⊢ₚ wlp θ (P /\ₚ Q). *)
+      (*   wlp θ P ∧ wlp θ Q ⊣⊢ wlp θ (P ∧ Q). *)
       (* Proof. firstorder. Qed. *)
 
       (* Lemma wp_or {w0 w1} (θ : Θ w0 w1) P Q : *)
-      (*   wp θ P \/ₚ wp θ Q ⊣⊢ₚ wp θ (P \/ₚ Q). *)
+      (*   wp θ P ∨ wp θ Q ⊣⊢ wp θ (P ∨ Q). *)
       (* Proof. firstorder. Qed. *)
 
-      Lemma wp_mono {w0 w1} (θ : Θ w0 w1) P Q:
-        wlp θ (interface.bi_wand P Q) ⊢ₚ interface.bi_wand (wp θ P) (wp θ Q).
+      Lemma wp_mono {w0 w1} (θ : Θ w0 w1) P Q :
+        wlp θ (P -∗ Q) ⊢ wp θ P -∗ wp θ Q.
       Proof. firstorder. Qed.
 
       Lemma wlp_mono {w0 w1} (θ : Θ w0 w1) P Q :
-        wlp θ (interface.bi_wand P Q) ⊢ₚ interface.bi_wand (wlp θ P) (wlp θ Q).
+        wlp θ (P -∗ Q) ⊢ wlp θ P -∗ wlp θ Q.
       Proof. firstorder. Qed.
 
       Lemma entails_wlp {w0 w1} (θ : Θ w0 w1) P Q :
-        (subst P θ ⊢ₚ Q) <-> (P ⊢ₚ wlp θ Q).
+        (P[θ] ⊢ Q) ↔ (P ⊢ wlp θ Q).
       Proof.
         unfold wlp; pred_unfold. split; intros HPQ.
         - intros ι0 HP ι1 <-. revert HP. apply HPQ.
@@ -552,7 +518,7 @@ Module Pred.
       Qed.
 
       Lemma entails_wp {w0 w1} (θ : Θ w0 w1) P Q :
-        (P ⊢ₚ subst Q θ) <-> (wp θ P ⊢ₚ Q).
+        (P ⊢ Q[θ]) ↔ (wp θ P ⊢ Q).
       Proof.
         unfold wp; pred_unfold. split; intros HPQ.
         - intros ι0 (ι1 & <- & HP). now apply HPQ.
@@ -560,7 +526,7 @@ Module Pred.
       Qed.
 
       Lemma wp_impl {w0 w1} (θ1 : Θ w0 w1) (P : Pred _) (Q : Pred _) :
-        (wp θ1 P ->ₚ Q) ⊣⊢ₚ wlp θ1 (P ->ₚ subst Q θ1).
+        (wp θ1 P → Q) ⊣⊢ wlp θ1 (P → Q[θ1]).
       Proof.
         unfold wp, wlp; pred_unfold. intros ι0; split.
         - intros H ι1 <- HP. apply H. now exists ι1.
@@ -568,15 +534,15 @@ Module Pred.
       Qed.
 
       Lemma subst_wlp {w0 w1} {θ : Θ w0 w1} (P : Pred w1) :
-        subst (wlp θ P) θ ⊢ₚ P.
+        (wlp θ P)[θ] ⊢ P.
       Proof. firstorder. Qed.
 
-      (* Lemma subst_wp {w0 w1} {θ : Θ w0 w1} (P : Pred w1) : *)
-      (*   P ⊢ₚ subst (wp θ P) θ. *)
-      (* Proof. firstorder. Qed. *)
+      Lemma subst_wp {w0 w1} {θ : Θ w0 w1} (P : Pred w1) :
+        P ⊢ (wp θ P)[θ].
+      Proof. firstorder. Qed.
 
       Lemma wlp_frame {w0 w1} (θ : Θ w0 w1) (P : Pred _) (Q : Pred _) :
-        P ->ₚ wlp θ Q ⊣⊢ₚ wlp θ (subst P θ ->ₚ Q).
+        (P → wlp θ Q) ⊣⊢ wlp θ (P[θ] → Q).
       Proof.
         unfold wlp; pred_unfold. intros ι; split.
         - intros H ι1 <- HP. now apply (H HP).
@@ -589,8 +555,8 @@ Module Pred.
 
     Lemma intro_wp_step' {Θ} {stepΘ : Step Θ} {lkStepΘ : LkStep Θ}
       {w α} (P : Pred w) (Q : Pred (w ، α)) (t : Ty) :
-      (subst P step ⊢ₚ lift t =ₚ @oty.evar _ α world.in_zero ->ₚ Q) ->
-      (P ⊢ₚ wp (step (Θ := Θ)) Q).
+      (P[step] ⊢ lift t ≈ oty.evar world.in_zero → Q) →
+      (P ⊢ wp (step (Θ := Θ)) Q).
     Proof.
       pred_unfold. intros H ι HP. set (ι1 := env.snoc ι α t). exists ι1.
       specialize (H ι1). rewrite inst_step in H |- *; cbn in *. intuition.
@@ -599,22 +565,22 @@ Module Pred.
     (* Better for iris proof mode. *)
     Lemma intro_wp_step {Θ} {stepΘ : Step Θ} {lkStepΘ : LkStep Θ}
       t {w α} (Q : Pred (w ، α)) :
-      wlp step (lift t =ₚ oty.evar world.in_zero ->ₚ Q) ⊢ₚ wp (step (Θ := Θ)) Q.
+      wlp step (lift t ≈ oty.evar world.in_zero → Q) ⊢ wp (step (Θ := Θ)) Q.
     Proof. apply (intro_wp_step' t). now rewrite subst_wlp. Qed.
 
     (* Lemma wp_split  {Θ : SUB} [w0 w1] (θ : Θ w0 w1) P : *)
-    (*   wp θ ⊤ₚ /\ₚ wlp θ P ⊢ₚ wp θ P. *)
-    (* Proof. now rewrite and_wp_l, subst_wlp, and_true_l. Qed. *)
+    (*   wp θ ⊤ ∧ wlp θ P ⊢ wp θ P. *)
+    (* Proof. now rewrite and_wp_l subst_wlp and_true_l. Qed. *)
 
     Lemma wp_hmap `{LkHMap Θ1 Θ2} [w0 w1] (θ : Θ1 w0 w1) P :
-      wp (hmap θ) P ⊣⊢ₚ wp θ P.
+      wp (hmap θ) P ⊣⊢ wp θ P.
     Proof.
       constructor. intros ι0; cbn. apply ex_iff_morphism.
       intro ι1. now rewrite inst_hmap.
     Qed.
 
     Lemma wlp_hmap `{LkHMap Θ1 Θ2} [w0 w1] (θ : Θ1 w0 w1) P :
-      wlp (hmap θ) P ⊣⊢ₚ wlp θ P.
+      wlp (hmap θ) P ⊣⊢ wlp θ P.
     Proof.
       constructor. intros ι0; cbn. apply all_iff_morphism.
       intro ι1. now rewrite inst_hmap.
@@ -622,16 +588,12 @@ Module Pred.
 
   End Sub.
 
-  Definition PBox {Θ} : ⊧ Box Θ Pred ⇢ Pred :=
-    fun w Q => (∀ₚ w' (θ : Θ w w'), Sub.wlp θ (Q w' θ))%P.
-  Notation "◼ Q" := (PBox Q%B) (at level 9, right associativity, format "◼ Q").
-
   Section InstPred.
     Import iris.bi.derived_laws iris.bi.interface.
 
     (* A type class for things that can be interpreted as a predicate. *)
     Class InstPred (A : OType) :=
-      instpred : ⊧ A ⇢ Pred.
+      instpred : ⊧ A ↠ Pred.
     #[global] Arguments instpred {_ _ _}.
 
     (* #[export] Instance instpred_option {A} `{ipA : InstPred A} : *)
@@ -642,17 +604,17 @@ Module Pred.
       fun w =>
         fix ip xs {struct xs} :=
         match xs with
-        | nil       => ⊤ₚ
-        | cons y ys => instpred y /\ₚ ip ys
-        end%P.
+        | nil       => ⊤
+        | cons y ys => instpred y ∧ ip ys
+        end%I.
     #[local] Instance instpred_prod_ty : InstPred (OTy * OTy) :=
-      fun w '(t1,t2) => eqₚ t1 t2.
+      fun w '(t1,t2) => oeq t1 t2.
     #[export] Instance instpred_unit : InstPred Unit :=
-      fun w _ => ⊤ₚ%P.
+      fun w _ => ⊤%I.
     #[global] Arguments instpred_unit [w] _ /.
 
     Lemma instpred_list_app {A} `{ipA : InstPred A} [w] (xs ys : List A w) :
-      instpred (xs ++ ys) ⊣⊢ₚ instpred xs /\ₚ instpred ys.
+      instpred (xs ++ ys) ⊣⊢ instpred xs ∧ instpred ys.
     Proof.
       induction xs; cbn.
       - now rewrite and_true_l.
@@ -661,7 +623,7 @@ Module Pred.
 
     Class InstPredSubst A {ipA : InstPred A} {subA : Subst A} :=
       instpred_subst [Θ : SUB] {w0 w1} (θ : Θ w0 w1) (a : A w0) :
-        instpred (subst a θ) ⊣⊢ₚ subst (instpred a) θ.
+        instpred a[θ] ⊣⊢ (instpred a)[θ].
     #[global] Arguments InstPredSubst _ {_ _}.
 
     #[export] Instance instpred_subst_list `{InstPredSubst A} :
@@ -677,29 +639,37 @@ Module Pred.
   End InstPred.
 
   Lemma pno_cycle {w} (t1 t2 : OTy w) (Hsub : oty.OTy_subterm t1 t2) :
-    t1 =ₚ t2 ⊢ₚ ⊥ₚ.
+    t1 ≈ t2 ⊢ ⊥.
   Proof.
     constructor. intros ι Heq. apply (inst_subterm ι) in Hsub.
     rewrite <- Heq in Hsub. now apply ty.no_cycle in Hsub.
   Qed.
 
-  Lemma eqₚ_insert {w} (G1 G2 : OEnv w) (x : string) (t1 t2 : OTy w) :
-    G1 =ₚ G2 /\ₚ t1 =ₚ t2 ⊢ₚ
-    insert (M := OEnv w) x t1 G1 =ₚ insert (M := OEnv w) x t2 G2.
+  Lemma oeq_insert {w} (G1 G2 : OEnv w) (x : string) (t1 t2 : OTy w) :
+    G1 ≈ G2 ∧ t1 ≈ t2 ⊢
+    insert (M := OEnv w) x t1 G1 ≈ insert (M := OEnv w) x t2 G2.
   Proof. pred_unfold. intros []. now f_equal. Qed.
 
-  Lemma eq_func {w} (s1 s2 t1 t2 : OTy w) :
-    oty.func s1 s2 =ₚ oty.func t1 t2 ⊣⊢ₚ (s1 =ₚ t1) /\ₚ (s2 =ₚ t2).
-  Proof. now rewrite peq_ty_noconfusion. Qed.
+  Lemma oeq_func {w} (s1 s2 t1 t2 : OTy w) :
+    oty.func s1 s2 ≈ oty.func t1 t2 ⊣⊢ (s1 ≈ t1) ∧ (s2 ≈ t2).
+  Proof. now rewrite oeq_ty_noconfusion. Qed.
 
-  #[export] Instance params_tpb : Params (@TPB) 1 := {}.
+  #[export] Instance params_tpb : Params (@otyping_decl) 1 := {}.
   #[export] Instance params_ifte : Params (@oexp.ifte) 1 := {}.
-  #[export] Instance params_eqₚ : Params (@eqₚ) 4 := {}.
+  #[export] Instance params_oeq : Params (@oeq) 4 := {}.
   #[export] Instance params_subst : Params (@subst) 4 := {}.
+
+  Definition PBox {Θ} : ⊧ Box Θ Pred ↠ Pred :=
+    fun w Q => (∀ w' (θ : Θ w w'), Sub.wlp θ (Q w' θ))%I.
+  Notation "◼ Q" := (PBox Q%B) (at level 9, right associativity, format "◼ Q").
 
   Section PBoxModality.
     Import iris.proofmode.tactics.
 
+    (* We instantiate the iris modality elimination machinery for the ◼ modality.
+       That means every time we have a hypothesis with that modality at the
+       head, we can eliminate it. Eliminating the modality from ◼P will simply
+       use P at the current world w, which is accessible as witnessed y refl. *)
     #[export] Instance elimpbox `{LkRefl Θ} (p : bool)
       {w} (P : ◻Pred w) (Q : Pred w) :
       ElimModal True p true ◼P (P w refl) Q Q.
@@ -709,8 +679,9 @@ Module Pred.
         now erewrite Sub.wlp_refl.
     Qed.
 
+    (* Substitution distributes over ◼. *)
     Lemma subst_pbox `{LkTrans Θ} [w] (Q : ◻Pred w) [w1] (θ1 : Θ w w1) :
-      (◼Q)[θ1] ⊢ₚ ◼(Q[θ1]).
+      (◼Q)[θ1] ⊢ ◼(Q[θ1]).
     Proof.
       constructor; intros ι1 HQ w2 θ2 ι2 <-.
       apply HQ. now rewrite inst_trans.
@@ -722,10 +693,14 @@ Module Pred.
 
     Context {Θ : SUB}.
 
+    (* We use the [IntoSubst] type class to perform logic programming that
+       will automatically push substitutions down. The idea is that [y] is
+       equivalent to [x] with the substitution [θ] applied. *)
     Class IntoSubst `{Inst T A, Subst T}
       [w0 w1] (θ : Θ w0 w1) (x : T w0) (y : T w1) : Prop :=
-      into_subst : forall ι : Assignment w1, inst (subst x θ) ι = inst y ι.
+      into_subst : ∀ ι : Assignment w1, inst (subst x θ) ι = inst y ι.
 
+    (* The default instance (with lower priority) simply applies [θ] to [t]. *)
     #[export] Instance into_subst_default `{Inst T A, Subst T}
       [w0 w1] (θ : Θ w0 w1) (t : T w0) : IntoSubst θ t (subst t θ) | 10.
     Proof. easy. Qed.
@@ -739,7 +714,7 @@ Module Pred.
       {subT : Subst T} {instLiftTA : InstLift T A} {instSubTA : InstSubst T A}
       [w0 w1] (θ : Θ w0 w1) (a : A) :
       IntoSubst θ (lift a) (lift a) | 0.
-    Proof. intros ι. now rewrite inst_subst, !inst_lift. Qed.
+    Proof. intros ι. now rewrite inst_subst !inst_lift. Qed.
 
     #[export] Instance into_subst_insert
       [w0 w1] (θ : Θ w0 w1) (G0 : OEnv w0) x (τ0 : OTy w0) G1 τ1
@@ -748,7 +723,7 @@ Module Pred.
     Proof.
       intros ι1. specialize (HG ι1). specialize (Hτ ι1).
       change_no_check (@gmap.gmap string _ _ (OTy ?w)) with (OEnv w).
-      rewrite subst_insert, !inst_insert. now f_equal.
+      rewrite subst_insert !inst_insert. now f_equal.
     Qed.
 
   End IntoSubst.
@@ -759,6 +734,10 @@ Module Pred.
 
     Context {Θ : SUB} [w0 w1] (θ : Θ w0 w1).
 
+    (* We instantiate the iris modality introduction machinery for the wlp
+       modality. The effect of introducing [wlp θ] is to run the substitution
+       [θ] over all hypotheses and eliminate [wlp θ] from the head of the
+       goal. *)
     Class IntoWlp (P : Pred w0) (Q : Pred w1) :=
       into_wlp : P ⊢ Sub.wlp θ Q.
 
@@ -783,19 +762,19 @@ Module Pred.
       IntoWlp ◼P ◼(fun _ θ2 => P _ (θ ⊙ θ2)) | 0.
     Proof. unfold IntoWlp. iIntros "H !>". now rewrite subst_pbox. Qed.
 
-    #[export] Instance into_wlp_tpb (G1 : OEnv w0) (e : Exp) (τ1 : OTy w0)
+    #[export] Instance into_wlp_typing (G1 : OEnv w0) (e : Exp) (τ1 : OTy w0)
       (ee1 : OExp w0) G2 τ2 ee2 (HG : IntoSubst θ G1 G2)
       (Hτ : IntoSubst θ τ1 τ2) (Hee : IntoSubst θ ee1 ee2) :
-      IntoWlp (TPB G1 e τ1 ee1) (TPB G2 e τ2 ee2) | 0.
+      IntoWlp (G1 |--ₚ e; τ1 ~> ee1) (G2 |--ₚ e; τ2 ~> ee2) | 0.
     Proof.
       constructor. intros ι0 HT ι1 <-. pred_unfold.
       specialize (HG ι1). specialize (Hτ ι1). specialize (Hee ι1).
       rewrite !inst_subst in HG, Hτ, Hee. congruence.
     Qed.
 
-    #[export] Instance into_wlp_eqp `{InstSubst T A}
-      (x1 x2 : T w0) (y1 y2 : T w1) (Hxy1 : IntoSubst θ x1 y1) (Hxy2 :IntoSubst θ x2 y2) :
-      IntoWlp (eqₚ x1 x2) (eqₚ y1 y2) | 0.
+    #[export] Instance into_wlp_eqp `{InstSubst T A} (x1 x2 : T w0)
+      (y1 y2 : T w1) (Hxy1 : IntoSubst θ x1 y1) (Hxy2 : IntoSubst θ x2 y2) :
+      IntoWlp (x1 ≈ x2) (y1 ≈ y2) | 0.
     Proof.
       constructor. pred_unfold. intros ι0 Heq ι1 ?Heq; cbn.
       specialize (Hxy1 ι1). specialize (Hxy2 ι1).
@@ -819,9 +798,9 @@ Module Pred.
     (@subst_refl OEnv _ _) (@subst_refl OTy _ _) (@subst_trans OEnv _ _)
     (@subst_trans OTy _ _) @Sub.wlp_refl @Sub.wlp_trans @Sub.wlp_true
     @Sub.wp_false @Sub.wp_refl @Sub.wp_trans @and_false_l @and_false_r
-    @and_true_l @and_true_r @eq_func @eqₚ_refl @impl_and @impl_false_l
+    @and_true_l @and_true_r @oeq_func @oeq_refl @impl_and @impl_false_l
     @impl_true_l @impl_true_r @lk_refl @lk_step @lk_trans @subst_and @subst_false
-    @subst_pred_refl @subst_pred_trans @subst_tpb @subst_true @trans_refl_r
+    @subst_pred_refl @subst_pred_trans @subst_typing @subst_true @trans_refl_r
     : predsimpl.
   Ltac predsimpl :=
     repeat
@@ -829,8 +808,8 @@ Module Pred.
        change_no_check (@gmap.gmap string _ _ (OTy ?w)) with (OEnv w) in *;
        repeat
          match goal with
-         | |- Sub.wp ?θ _ ⊣⊢ₚ Sub.wp ?θ _ => apply Sub.proper_wp_bientails
-         | |- Sub.wlp ?θ _ ⊣⊢ₚ Sub.wlp ?θ _ => apply Sub.proper_wlp_bientails
+         | |- Sub.wp ?θ _ ⊣⊢ Sub.wp ?θ _ => apply Sub.proper_wp_bientails
+         | |- Sub.wlp ?θ _ ⊣⊢ Sub.wlp ?θ _ => apply Sub.proper_wlp_bientails
          end;
        try easy; repeat rewrite_db predsimpl; auto 1 with typeclass_instances;
        repeat
