theories/Gen/Synthesise.v
@@ -44,7 +44,7 @@ Section Generator.
     {reflTransΘ: ReflTrans Θ}.
   Context `{pureM:Pure M, bindM:Bind Θ M, failM:Fail M, tcM:TypeCheckM M}.
 
-  Definition osynth : Exp -> ⊧ OEnv ⇢ M (OTy * OExp) :=
+  Definition osynth : Exp -> ⊧ OEnv ↠ M (OTy * OExp) :=
     fix osynth e {w} Γ :=
       match e with
       | exp.var x =>
@@ -76,17 +76,14 @@ Section Generator.
           pure (t2[_], oexp.app e1'[_] e2'[_])
       end.
 
-  Import Pred Pred.notations Pred.proofmode iris.proofmode.tactics.
-  Open Scope pred_scope.
-
   Context {wpM : WeakestPre Θ M} {wlpM : WeakestLiberalPre Θ M}
     {tcLogicM : TypeCheckLogicM Θ M}.
 
-  Definition otyping_algo : ⊧ OEnv ⇢ Const Exp ⇢ OTy ⇢ OExp ⇢ Pred :=
+  Definition otyping_algo : ⊧ OEnv ↠ Const Exp ↠ OTy ↠ OExp ↠ Pred :=
     fun w0 G0 e t0 e0 =>
     WP (osynth e G0)
       (fun w1 (θ1 : Θ w0 w1) '(t1,e1) =>
-         t0[θ1] =ₚ t1 /\ₚ e0[θ1] =ₚ e1).
+         t0[θ1] ≈ t1 ∧ e0[θ1] ≈ e1)%I.
   Notation "Γ |--ₐ e ∷ t ~> e'" := (otyping_algo Γ e t e') (at level 75).
 
   Goal False. Proof.
@@ -96,7 +93,7 @@ Section Generator.
       |- environments.envs_entails _ (WLP (osynth ?e ?G) _) =>
         iApply (wlp_mono' $! (IH _ G));
         iIntros (?w ?θ) "!>"; iIntros ([?t ?e']) "#?"; clear IH
-    | |- environments.envs_entails _ (TPB _ _ _ _) =>
+    | |- environments.envs_entails _ (otyping_decl _ _ _ _) =>
         iStopProof; pred_unfold;
         intuition (subst; econstructor; eauto; fail)
     end.
@@ -197,7 +194,7 @@ Section Generator.
   Qed.
 
   Lemma osoundness (e : Exp) {w} (Γ : OEnv w) τ e' :
-    Γ |--ₐ e ∷ τ ~> e'  ⊢ₚ  Γ |--ₚ e; τ ~> e'.
+    Γ |--ₐ e ∷ τ ~> e'  ⊢  Γ |--ₚ e; τ ~> e'.
   Proof.
     iStartProof. rewrite wand_is_impl. iApply wp_impl.
     iApply (wlp_mono' $! (@osoundness_aux e w Γ)).
@@ -206,9 +203,9 @@ Section Generator.
   Qed.
 
   Lemma ocompleteness_aux {G e t ee} (T : G |-- e ∷ t ~> ee) :
-    ∀ w0 (G0 : OEnv w0), ⊢ lift G =ₚ G0 →
+    ∀ w0 (G0 : OEnv w0), ⊢ lift G ≈ G0 →
       WP (osynth e G0)
-          (fun _ _ '(t',e') => lift t =ₚ t' /\ₚ Open.pure ee =ₚ e')%P.
+          (fun _ _ '(t',e') => lift t ≈ t' ∧ Open.pure ee ≈ e')%I.
   Proof.
     induction T; cbn; intros w0 G0; iStartProof; wpauto.
     destruct (G0 !! x) eqn:HGx; wpauto; iStopProof; pred_unfold;
@@ -216,7 +213,7 @@ Section Generator.
   Qed.
 
   Lemma ocompleteness {w} (Γ : OEnv w) (e : Exp) (τ : OTy w) (e' : OExp w) :
-    Γ |--ₚ e; τ ~> e'  ⊢ₚ  Γ |--ₐ e ∷ τ ~> e'.
+    Γ |--ₚ e; τ ~> e'  ⊢  Γ |--ₐ e ∷ τ ~> e'.
   Proof.
     pred_unfold. intros ι HT.
     destruct (ocompleteness_aux HT Γ) as [Hcompl].
@@ -228,7 +225,7 @@ Section Generator.
   Qed.
 
   Lemma ocorrectness {w} (Γ : OEnv w) (e : Exp) (τ : OTy w) (e' : OExp w) :
-    Γ |--ₚ e; τ ~> e'  ⊣⊢ₚ  Γ |--ₐ e ∷ τ ~> e'.
+    Γ |--ₚ e; τ ~> e'  ⊣⊢  Γ |--ₐ e ∷ τ ~> e'.
   Proof. iSplit. iApply ocompleteness. iApply osoundness. Qed.
 
 End Generator.
