theories/Related/Gen/Synthesise.v
@@ -103,7 +103,7 @@ Section Relatedness.
 
   Lemma generate_correct_logrel `{!Shallow.Monad.Interface.TypeCheckLogicM SM}
     {w} (Γ : OEnv w) (e : Exp) (τ : OTy w) (e' : OExp w) :
-    otyping_algo (M := DM) Γ e τ e'  ⊣⊢ₚ  Γ |--ₚ e; τ ~> e'.
+    otyping_algo (M := DM) Γ e τ e'  ⊣⊢  Γ |--ₚ e; τ ~> e'.
   Proof.
     constructor. intros ι. simpl. rewrite correctness.
     now apply relatedness_of_algo_typing.
